SlowTest/DLL-int.dfy
@@ -96,12 +96,12 @@ predicate Invs<A>(nodes:seq<Node<A>>, freeStack:int, s:seq<A>, f:seq<int>, g:seq
   && (forall p {:trigger g[p]} {:trigger f[g[p]]} {:trigger s[g[p]]} :: 
     0 <= p < |g| && sentinel <= g[p] ==>
       (0 <= g[p] ==> f[g[p]] == p && nodes[p].data == Some(s[g[p]])) )
-  && (forall p {:trigger g[p]} {:trigger nodes[p].next} ::
+  && (forall p {:trigger g[p]} {:trigger nodes[p]} ::
     0 <= p < |g| && sentinel <= g[p] ==>
       nodes[p].next == (
         if g[p] + 1 < |f| then f[g[p] + 1] // nonlast.next or sentinel.next
         else 0) ) // last.next == sentinel or sentinel.next == sentinel
-  && (forall p  {:trigger g[p]} {:trigger nodes[p].prev} ::
+  && (forall p  {:trigger g[p]} {:trigger nodes[p]} ::
     0 <= p < |g| && sentinel <= g[p] ==>
     && nodes[p].prev == (
       if g[p] > 0 then f[g[p] - 1] // nonfirst.prev
